New algebraic laws for the lifted substitution in designs theory
git-svn-id: orca@290

WP1-Programming-Languages-Semantics/WP11-C-semantics/src/IMP-Lenses/theories/utp_abrupt_designs.thy
@@ -13,11 +13,11 @@ text {*In order to record the interaction of a sequential C program with its exe
 
 *}
 
-alphabet  'a cp_abr = des_vars +
+alphabet  cp_abr = des_vars +
   abrupt:: bool
-  abrupt_aux :: "'a option" (*store the reason of the abrupt termination*)
+ (* abrupt_aux :: "'a option" store the reason of the abrupt termination*)
   (*wait :: bool*)
-
+update_uexpr_rep_eq_thms
 declare cp_abr.splits [alpha_splits]
 
 subsubsection {*Alphabet proofs*}
@@ -32,14 +32,14 @@ text {*
 *}
 
 interpretation cp_abr:
-  lens_interp "\<lambda> (ok, r) . (ok, abrupt\<^sub>v r, abrupt_aux\<^sub>v r, more r)"
+  lens_interp "\<lambda> (ok, r) . (ok, abrupt\<^sub>v r, more r)"
 apply (unfold_locales)
 apply (rule injI)
 apply (clarsimp)
 done
 
 interpretation cp_abr_rel: lens_interp "\<lambda>(ok, ok', r, r').
-  (ok, ok', abrupt\<^sub>v r, abrupt\<^sub>v r', abrupt_aux\<^sub>v r, abrupt_aux\<^sub>v r', more r, more r')"
+  (ok, ok', abrupt\<^sub>v r, abrupt\<^sub>v r', more r, more r')"
 apply (unfold_locales)
 apply (rule injI)
 apply (clarsimp)
@@ -48,16 +48,16 @@ done
 
 subsubsection {*Type lifting*}
 
-type_synonym  ('a, '\<alpha>) cpa = "('a, '\<alpha>) cp_abr_scheme des"
-type_synonym ('a,'\<alpha>,'\<beta>) rel_cpa  = "(('a, '\<alpha>) cpa, ('a, '\<beta>) cpa) rel"
-type_synonym ('a, '\<alpha>) hrel_cpa  = "(('a, '\<alpha>) cpa) hrel"
+type_synonym  ('\<alpha>) cpa = "('\<alpha>) cp_abr_scheme des"
+type_synonym ('\<alpha>,'\<beta>) rel_cpa  = "(('\<alpha>) cpa, ('\<beta>) cpa) rel"
+type_synonym ('\<alpha>) hrel_cpa  = "(('\<alpha>) cpa) hrel"
 
 subsubsection {*Syntactic type setup*}
 
 translations
-  (type) "('a, '\<alpha>) cpa" <= (type) " ('a, '\<alpha>) cp_abr_scheme des"
-  (type) "('a, '\<alpha>) cpa" <= (type) " ('a, '\<alpha>) cp_abr_ext des"
-  (type) "('a,'\<alpha>,'\<beta>) rel_cpa" <= (type) "(('a, '\<alpha>) cpa, (_, '\<beta>) cpa) rel"
+  (type) "('\<alpha>) cpa" <= (type) " ('\<alpha>) cp_abr_scheme des"
+  (type) "('\<alpha>) cpa" <= (type) " ('\<alpha>) cp_abr_ext des"
+  (type) "('\<alpha>,'\<beta>) rel_cpa" <= (type) "(('\<alpha>) cpa, ('\<beta>) cpa) rel"
 
 notation cp_abr_child_lens\<^sub>a ("\<Sigma>\<^sub>a\<^sub>b\<^sub>r")
 notation cp_abr_child_lens ("\<Sigma>\<^sub>A\<^sub>B\<^sub>R")
@@ -69,17 +69,10 @@ translations
   "_svid_st_alpha" => "CONST cp_abr_child_lens"
    "_svid_st_a" => "CONST cp_abr_child_lens\<^sub>a"
 
-lemma cvars_ord [usubst]:
-  "$ok \<prec>\<^sub>v $ok\<acute>" "$abrupt \<prec>\<^sub>v $abrupt\<acute>" 
-  "$ok \<prec>\<^sub>v $abrupt\<acute>" "$ok \<prec>\<^sub>v $abrupt" "$ok\<acute> \<prec>\<^sub>v $abrupt\<acute>" "$ok\<acute> \<prec>\<^sub>v $abrupt" 
-  "$ok \<prec>\<^sub>v $abrupt_aux\<acute>" "$ok \<prec>\<^sub>v $abrupt_aux" "$ok\<acute> \<prec>\<^sub>v $abrupt_aux\<acute>" "$ok\<acute> \<prec>\<^sub>v $abrupt_aux"
-  "$abrupt \<prec>\<^sub>v $abrupt_aux\<acute>" "$abrupt \<prec>\<^sub>v $abrupt_aux" "$abrupt\<acute> \<prec>\<^sub>v $abrupt_aux\<acute>" "$abrupt\<acute> \<prec>\<^sub>v $abrupt_aux"
-  by (simp_all add: var_name_ord_def)
-
-abbreviation abrupt_f::"('a,'\<alpha>, '\<beta>) rel_cpa \<Rightarrow> ('a, '\<alpha>, '\<beta>) rel_cpa"
+abbreviation abrupt_f::"('\<alpha>, '\<beta>) rel_cpa \<Rightarrow> ('\<alpha>, '\<beta>) rel_cpa"
 where "abrupt_f R \<equiv> R\<lbrakk>false/$abrupt\<rbrakk>"
 
-abbreviation abrupt_t::"('a,'\<alpha>, '\<beta>) rel_cpa \<Rightarrow> ('a,'\<alpha>, '\<beta>) rel_cpa"
+abbreviation abrupt_t::"('\<alpha>, '\<beta>) rel_cpa \<Rightarrow> ('\<alpha>, '\<beta>) rel_cpa"
 where "abrupt_t R \<equiv> R\<lbrakk>true/$abrupt\<rbrakk>"
 
 syntax
@@ -93,50 +86,55 @@ translations
   "P \<^sub>a\<^sub>t" \<rightleftharpoons> "CONST usubst (CONST subst_upd CONST id (CONST ivar CONST abrupt) true) P"
   "\<top>\<^sub>A\<^sub>B\<^sub>R" => "CONST conj_upred 
             (CONST not_upred (CONST utp_expr.var (CONST ivar CONST ok))) 
-            (CONST conj_upred (CONST not_upred (CONST utp_expr.var (CONST ivar CONST abrupt)))
-                              (CONST eq_upred  (CONST utp_expr.var (CONST ivar CONST abrupt_aux))
-                                               (CONST utp_expr.lit (CONST None))))"
+            (CONST not_upred (CONST utp_expr.var (CONST ivar CONST abrupt)))
+                              "
   "\<bottom>\<^sub>A\<^sub>B\<^sub>R" => "true"
 
-lemma "\<top>\<^sub>A\<^sub>B\<^sub>R = ((\<not> $ok) \<and> (\<not> $abrupt) \<and> ($abrupt_aux =\<^sub>u \<guillemotleft>None\<guillemotright>))"
+lemma "\<top>\<^sub>A\<^sub>B\<^sub>R = ((\<not> $ok) \<and> (\<not> $abrupt))"
   by auto
+
+subsection {*Substitution lift and drop*}
+
+abbreviation lift_rel_usubst_cpa ("\<lceil>_\<rceil>\<^sub>S\<^sub>A\<^sub>B\<^sub>R")
+where "\<lceil>\<sigma>\<rceil>\<^sub>S\<^sub>A\<^sub>B\<^sub>R \<equiv> \<sigma> \<oplus>\<^sub>s (\<Sigma>\<^sub>A\<^sub>B\<^sub>R \<times>\<^sub>L \<Sigma>\<^sub>A\<^sub>B\<^sub>R)"
+
+abbreviation lift_usubst_cpa ("\<lceil>_\<rceil>\<^sub>s\<^sub>A\<^sub>B\<^sub>R")
+where "\<lceil>\<sigma>\<rceil>\<^sub>s\<^sub>A\<^sub>B\<^sub>R \<equiv> \<lceil>\<lceil>\<sigma>\<rceil>\<^sub>s\<rceil>\<^sub>S\<^sub>A\<^sub>B\<^sub>R"
+
+abbreviation drop_cpa_rel_usubst ("\<lfloor>_\<rfloor>\<^sub>S\<^sub>A\<^sub>B\<^sub>R")
+where "\<lfloor>\<sigma>\<rfloor>\<^sub>S\<^sub>A\<^sub>B\<^sub>R \<equiv> \<sigma> \<restriction>\<^sub>s (\<Sigma>\<^sub>A\<^sub>B\<^sub>R \<times>\<^sub>L \<Sigma>\<^sub>A\<^sub>B\<^sub>R)"
+
+abbreviation drop_cpa_usubst ("\<lfloor>_\<rfloor>\<^sub>s\<^sub>A\<^sub>B\<^sub>R")
+where "\<lfloor>\<sigma>\<rfloor>\<^sub>s\<^sub>A\<^sub>B\<^sub>R \<equiv> \<lfloor>\<lfloor>\<sigma>\<rfloor>\<^sub>S\<^sub>A\<^sub>B\<^sub>R\<rfloor>\<^sub>s"
 
 subsection {*UTP-Relations lift and drop*}
 
-abbreviation lift_desr ("\<lceil>_\<rceil>\<^sub>A\<^sub>B\<^sub>R")
+abbreviation lift_rel_uexpr_cpa ("\<lceil>_\<rceil>\<^sub>A\<^sub>B\<^sub>R")
 where "\<lceil>P\<rceil>\<^sub>A\<^sub>B\<^sub>R \<equiv> P \<oplus>\<^sub>p (\<Sigma>\<^sub>A\<^sub>B\<^sub>R \<times>\<^sub>L \<Sigma>\<^sub>A\<^sub>B\<^sub>R)"
 
-abbreviation lift_pre_desr ("\<lceil>_\<rceil>\<^sub>A\<^sub>B\<^sub>R\<^sub><")
+abbreviation lift_pre_uexpr_cpa ("\<lceil>_\<rceil>\<^sub>A\<^sub>B\<^sub>R\<^sub><")
 where "\<lceil>p\<rceil>\<^sub>A\<^sub>B\<^sub>R\<^sub>< \<equiv> \<lceil>\<lceil>p\<rceil>\<^sub><\<rceil>\<^sub>A\<^sub>B\<^sub>R"
 
-abbreviation lift_post_desr ("\<lceil>_\<rceil>\<^sub>A\<^sub>B\<^sub>R\<^sub>>")
+abbreviation lift_post_uexpr_cpa ("\<lceil>_\<rceil>\<^sub>A\<^sub>B\<^sub>R\<^sub>>")
 where "\<lceil>p\<rceil>\<^sub>A\<^sub>B\<^sub>R\<^sub>> \<equiv> \<lceil>\<lceil>p\<rceil>\<^sub>>\<rceil>\<^sub>A\<^sub>B\<^sub>R"
 
-abbreviation drop_desr ("\<lfloor>_\<rfloor>\<^sub>A\<^sub>B\<^sub>R")
+abbreviation drop_cpa_rel_uexpr ("\<lfloor>_\<rfloor>\<^sub>A\<^sub>B\<^sub>R")
 where "\<lfloor>P\<rfloor>\<^sub>A\<^sub>B\<^sub>R \<equiv> P \<restriction>\<^sub>p (\<Sigma>\<^sub>A\<^sub>B\<^sub>R \<times>\<^sub>L \<Sigma>\<^sub>A\<^sub>B\<^sub>R)"
 
+abbreviation drop_cpa_pre_uexpr ("\<lfloor>_\<rfloor>\<^sub><\<^sub>A\<^sub>B\<^sub>R")
+where "\<lfloor>P\<rfloor>\<^sub><\<^sub>A\<^sub>B\<^sub>R \<equiv> \<lfloor>\<lfloor>P\<rfloor>\<^sub>A\<^sub>B\<^sub>R\<rfloor>\<^sub><"
+
+abbreviation drop_cpa_post_uexpr ("\<lfloor>_\<rfloor>\<^sub>>\<^sub>A\<^sub>B\<^sub>R")
+where "\<lfloor>P\<rfloor>\<^sub>>\<^sub>A\<^sub>B\<^sub>R \<equiv> \<lfloor>\<lfloor>P\<rfloor>\<^sub>A\<^sub>B\<^sub>R\<rfloor>\<^sub>>"
 
 subsection {* Reactive lemmas *}
 
-lemma unrest_ok_lift_rea [unrest]:
-  "$ok \<sharp> \<lceil>P\<rceil>\<^sub>A\<^sub>B\<^sub>R" "$ok\<acute> \<sharp> \<lceil>P\<rceil>\<^sub>A\<^sub>B\<^sub>R"
-  by (pred_auto)+
-
-lemma unrest_abrupt_lift_rea [unrest]:
-  "$abrupt \<sharp> \<lceil>P\<rceil>\<^sub>A\<^sub>B\<^sub>R" "$abrupt\<acute> \<sharp> \<lceil>P\<rceil>\<^sub>A\<^sub>B\<^sub>R"
-  by (pred_auto)+
-
-lemma seqr_abrupt_true [usubst]: "(P ;; Q) \<^sub>a\<^sub>t = (P \<^sub>a\<^sub>t ;; Q)"
-  by (rel_auto)
-
-lemma seqr_abrupt_false [usubst]: "(P ;; Q) \<^sub>a\<^sub>f = (P \<^sub>a\<^sub>f ;; Q)"
-  by (rel_auto)
 
 subsection{*Healthiness conditions*}
 
 text {*Programs in fault or abrupt or stuck state do not progress*}
 definition C3_abr_def [upred_defs]: 
-  "C3_abr(P) = (P \<triangleleft> \<not>$abrupt \<and> $abrupt_aux =\<^sub>u \<guillemotleft>None\<guillemotright> \<triangleright> II)"
+  "C3_abr(P) = (P \<triangleleft> \<not>$abrupt \<triangleright> II)"
 
 abbreviation
  "Simpl\<^sub>A\<^sub>B\<^sub>R P \<equiv> C3_abr(\<lceil>true\<rceil>\<^sub>A\<^sub>B\<^sub>R \<turnstile> (P))"
@@ -154,45 +152,45 @@ text{*We introduce the known control-flow statements for C. Our semantics is res
     Thus it capture Simpl semantics.
     *}
 
-
-definition skip_abr :: "('a, '\<alpha>) hrel_cpa" ("SKIP\<^sub>A\<^sub>B\<^sub>R")
+definition skip_abr :: "('\<alpha>) hrel_cpa" ("SKIP\<^sub>A\<^sub>B\<^sub>R")
 where [urel_defs]:
-  "SKIP\<^sub>A\<^sub>B\<^sub>R = Simpl\<^sub>A\<^sub>B\<^sub>R (\<not>$abrupt\<acute> \<and> $abrupt_aux\<acute> =\<^sub>u \<guillemotleft>None\<guillemotright> \<and> \<lceil>II\<rceil>\<^sub>A\<^sub>B\<^sub>R)"
-
-definition assigns_c :: " '\<alpha> usubst \<Rightarrow> ('a, '\<alpha>) hrel_cpa" ("\<langle>_\<rangle>\<^sub>A\<^sub>B\<^sub>R")
-where [urel_defs]: 
-  "assigns_c \<sigma> = Simpl\<^sub>A\<^sub>B\<^sub>R(\<not>$abrupt\<acute> \<and> $abrupt_aux\<acute> =\<^sub>u \<guillemotleft>None\<guillemotright> \<and> \<lceil>\<langle>\<sigma>\<rangle>\<^sub>a\<rceil>\<^sub>A\<^sub>B\<^sub>R)"
+  "SKIP\<^sub>A\<^sub>B\<^sub>R = Simpl\<^sub>A\<^sub>B\<^sub>R (\<not>$abrupt\<acute> \<and> \<lceil>II\<rceil>\<^sub>A\<^sub>B\<^sub>R)"
 
 subsection{*THROW*}
 
-definition throw_abr :: "('a, '\<alpha>) hrel_cpa" ("THROW\<^sub>A\<^sub>B\<^sub>R")
+definition throw_abr :: "('\<alpha>) hrel_cpa" ("THROW\<^sub>A\<^sub>B\<^sub>R")
 where [urel_defs]: 
-  "THROW\<^sub>A\<^sub>B\<^sub>R = Simpl\<^sub>A\<^sub>B\<^sub>R ($abrupt\<acute> \<and> $abrupt_aux\<acute> =\<^sub>u \<guillemotleft>None\<guillemotright> \<and> \<lceil>II\<rceil>\<^sub>A\<^sub>B\<^sub>R)"
+  "THROW\<^sub>A\<^sub>B\<^sub>R = Simpl\<^sub>A\<^sub>B\<^sub>R ($abrupt\<acute> \<and> \<lceil>II\<rceil>\<^sub>A\<^sub>B\<^sub>R)"
+
+definition assigns_abr :: " '\<alpha> usubst \<Rightarrow> ('\<alpha>) hrel_cpa" ("\<langle>_\<rangle>\<^sub>A\<^sub>B\<^sub>R")
+where [urel_defs]: 
+  "assigns_abr \<sigma> = Simpl\<^sub>A\<^sub>B\<^sub>R((\<not>$abrupt\<acute>) \<and> \<lceil>\<langle>\<sigma>\<rangle>\<^sub>a\<rceil>\<^sub>A\<^sub>B\<^sub>R)"
 
 subsection{*Conditional*}
 
-abbreviation If_abr :: "'\<alpha> cond \<Rightarrow> ('a, '\<alpha>) hrel_cpa \<Rightarrow> ('a, '\<alpha>) hrel_cpa \<Rightarrow> ('a, '\<alpha>) hrel_cpa" ("bif (_)/ then (_) else (_) eif")where
+abbreviation If_abr :: "'\<alpha> cond \<Rightarrow> ('\<alpha>) hrel_cpa \<Rightarrow> ('\<alpha>) hrel_cpa \<Rightarrow> ('\<alpha>) hrel_cpa" ("bif (_)/ then (_) else (_) eif")where
   "bif b then P else Q eif \<equiv> Simpl\<^sub>A\<^sub>B\<^sub>R (P \<triangleleft> \<lceil>b\<rceil>\<^sub>A\<^sub>B\<^sub>R\<^sub>< \<triangleright> Q)"
 
 subsection{*assert and assume*}
 
-definition rassume_abr :: "'\<alpha> upred \<Rightarrow> ('a, '\<alpha>) hrel_cpa" ("_\<^sup>\<top>\<^sup>C" [999] 999) where
+definition rassume_abr :: "'\<alpha> upred \<Rightarrow> ('\<alpha>) hrel_cpa" ("_\<^sup>\<top>\<^sup>C" [999] 999) where
 [urel_defs]: "rassume_abr c = (bif c then SKIP\<^sub>A\<^sub>B\<^sub>R else \<top>\<^sub>A\<^sub>B\<^sub>R eif)"
 
-definition rassert_abr :: "'\<alpha> upred \<Rightarrow> ('a, '\<alpha>) hrel_cpa" ("_\<^sub>\<bottom>\<^sub>C" [999] 999) where
+definition rassert_abr :: "'\<alpha> upred \<Rightarrow> ('\<alpha>) hrel_cpa" ("_\<^sub>\<bottom>\<^sub>C" [999] 999) where
 [urel_defs]: "rassert_abr c = (bif c then SKIP\<^sub>A\<^sub>B\<^sub>R else \<bottom>\<^sub>A\<^sub>B\<^sub>R eif)"
 
 subsection{*Exceptions*}
 
-abbreviation catch_abr :: "('a, '\<alpha>) hrel_cpa \<Rightarrow> ('a, '\<alpha>) hrel_cpa \<Rightarrow> ('a, '\<alpha>) hrel_cpa" ("try (_) catch /(_) end")
-where "try P catch Q end \<equiv> Simpl\<^sub>A\<^sub>B\<^sub>R (P ;; ((abrupt:== (\<not> &abrupt) ;;Q) \<triangleleft> $abrupt \<triangleright> II))"
+abbreviation catch_abr :: "('\<alpha>) hrel_cpa \<Rightarrow> ('\<alpha>) hrel_cpa \<Rightarrow> ('\<alpha>) hrel_cpa" ("try (_) catch /(_) end")
+where "try P catch Q end \<equiv> Simpl\<^sub>A\<^sub>B\<^sub>R (P ;; ((abrupt:== (\<not> &abrupt) ;; Q) \<triangleleft> $abrupt \<triangleright> II))"
 
 subsection{*Scoping*}
 
 definition block_abr ("bob INIT (_) BODY /(_) RESTORE /(_) RETURN/(_) eob") where
 [urel_defs]:
   "bob INIT init BODY body RESTORE restore RETURN return eob= 
-    Simpl\<^sub>A\<^sub>B\<^sub>R (Abs_uexpr (\<lambda>(s, s'). 
+     Simpl\<^sub>A\<^sub>B\<^sub>R
+    (Abs_uexpr (\<lambda>(s, s'). 
      \<lbrakk>init ;; body ;; Abs_uexpr (\<lambda>(t, t').
                        \<lbrakk>(abrupt:== (\<not> &abrupt) ;;restore (s, s') (t, t');; THROW\<^sub>A\<^sub>B\<^sub>R) \<triangleleft> $abrupt \<triangleright> II;; 
          restore (s, s') (t, t');; return(s, s') (t, t')\<rbrakk>\<^sub>e (t, t'))\<rbrakk>\<^sub>e (s, s')))" 
@@ -200,17 +198,17 @@ definition block_abr ("bob INIT (_) BODY /(_) RESTORE /(_) RETURN/(_) eob") wher
 subsection{*Loops*}
 purge_notation while ("while\<^sup>\<top> _ do _ od")
 
-definition While :: "'\<alpha> cond \<Rightarrow> ('a, '\<alpha>) hrel_cpa \<Rightarrow> ('a, '\<alpha>) hrel_cpa" ("while\<^sup>\<top> _ do _ od") where
+definition While :: "'\<alpha> cond \<Rightarrow> ('\<alpha>) hrel_cpa \<Rightarrow> ('\<alpha>) hrel_cpa" ("while\<^sup>\<top> _ do _ od") where
 "While b C = (\<nu> X \<bullet> bif b then (C ;; X) else SKIP\<^sub>A\<^sub>B\<^sub>R eif)"
 
 purge_notation while_top ("while _ do _ od")
 
-abbreviation While_top :: "'\<alpha> cond \<Rightarrow> ('a, '\<alpha>) hrel_cpa \<Rightarrow> ('a, '\<alpha>) hrel_cpa" ("while _ do _ od") where
+abbreviation While_top :: "'\<alpha> cond \<Rightarrow> ('\<alpha>) hrel_cpa \<Rightarrow> ('\<alpha>) hrel_cpa" ("while _ do _ od") where
 "while b do P od \<equiv> while\<^sup>\<top> b do P od"
 
 purge_notation while_bot ("while\<^sub>\<bottom> _ do _ od")
 
-definition While_bot :: "'\<alpha> cond \<Rightarrow> ('a, '\<alpha>) hrel_cpa \<Rightarrow> ('a, '\<alpha>) hrel_cpa" ("while\<^sub>\<bottom> _ do _ od") where
+definition While_bot :: "'\<alpha> cond \<Rightarrow> ('\<alpha>) hrel_cpa \<Rightarrow> ('\<alpha>) hrel_cpa" ("while\<^sub>\<bottom> _ do _ od") where
 "while\<^sub>\<bottom> b do P od =  (\<mu> X \<bullet> bif b then (P ;; X) else SKIP\<^sub>A\<^sub>B\<^sub>R eif)"
 
 subsection{*While-loop inv*}
@@ -218,7 +216,7 @@ text {* While loops with invariant decoration *}
 
 purge_notation while_inv ("while _ invr _ do _ od" 70)
 
-definition While_inv :: "'\<alpha> cond \<Rightarrow> '\<alpha> cond \<Rightarrow> ('a, '\<alpha>) hrel_cpa \<Rightarrow> ('a, '\<alpha>) hrel_cpa" ("while _ invr _ do _ od" 70) where
+definition While_inv :: "'\<alpha> cond \<Rightarrow> '\<alpha> cond \<Rightarrow> ('\<alpha>) hrel_cpa \<Rightarrow> ('\<alpha>) hrel_cpa" ("while _ invr _ do _ od" 70) where
 "while b invr p do S od = while b do S od"
 
 declare While_def [urel_defs]
@@ -227,12 +225,12 @@ declare While_bot_def [urel_defs]
 
 
 syntax
-  "_assignmentc" :: "svid_list \<Rightarrow> uexprs \<Rightarrow> logic"  (infixr "\<Midarrow>" 55)
+  "_assignmentabr" :: "svid_list \<Rightarrow> uexprs \<Rightarrow> logic"  (infixr "\<Midarrow>" 55)
 
 translations
-  "_assignmentc xs vs" => "CONST assigns_c (_mk_usubst (CONST id) xs vs)"
-  "x \<Midarrow> v" <= "CONST assigns_c (CONST subst_upd (CONST id) (CONST svar x) v)"
-  "x \<Midarrow> v" <= "CONST assigns_c (CONST subst_upd (CONST id) x v)"
-  "x,y \<Midarrow> u,v" <= "CONST assigns_c (CONST subst_upd (CONST subst_upd (CONST id) (CONST svar x) u) (CONST svar y) v)"
+  "_assignmentabr xs vs" => "CONST assigns_abr (_mk_usubst (CONST id) xs vs)"
+  "x \<Midarrow> v" <= "CONST assigns_abr (CONST subst_upd (CONST id) (CONST svar x) v)"
+  "x \<Midarrow> v" <= "CONST assigns_abr (CONST subst_upd (CONST id) x v)"
+  "x,y \<Midarrow> u,v" <= "CONST assigns_abr (CONST subst_upd (CONST subst_upd (CONST id) (CONST svar x) u) (CONST svar y) v)"
 
 end
