WP1-Programming-Languages-Semantics/WP11-C-semantics/src/IMP-Lenses/hoare/algebraic_laws_abrupt.thy
@@ -8,6 +8,18 @@ named_theorems symbolic_exec_cp
 
 subsection"Throw"
 
+lemma throw_not_ok_left_zero[simp]: 
+  "((\<not>$ok) ;; THROW\<^sub>A\<^sub>B\<^sub>R) = (\<not>$ok)" 
+  by rel_auto
+
+lemma throw_abr_left_zero[simp]: 
+  "($aburpt ;; THROW\<^sub>A\<^sub>B\<^sub>R) = $aburpt" 
+  by rel_auto 
+
+lemma throw_bot_left_zero[simp]: 
+  "(\<top>\<^sub>A\<^sub>B\<^sub>R ;; THROW\<^sub>A\<^sub>B\<^sub>R) = (\<top>\<^sub>A\<^sub>B\<^sub>R)" 
+  by rel_auto
+
 lemma throw_left_zero[simp]: 
   "(THROW\<^sub>A\<^sub>B\<^sub>R ;; Simpl\<^sub>A\<^sub>B\<^sub>R (P)) = THROW\<^sub>A\<^sub>B\<^sub>R" 
   by rel_auto 
@@ -20,7 +32,6 @@ lemma throw_right_zero_skip_abr[simp]:
   "(SKIP\<^sub>A\<^sub>B\<^sub>R ;; THROW\<^sub>A\<^sub>B\<^sub>R) = THROW\<^sub>A\<^sub>B\<^sub>R" 
   by rel_auto 
 
-
 lemma "try THROW\<^sub>A\<^sub>B\<^sub>R;; Simpl\<^sub>A\<^sub>B\<^sub>R P catch Simpl\<^sub>A\<^sub>B\<^sub>R Q end = Simpl\<^sub>A\<^sub>B\<^sub>R Q"
   by rel_auto (metis (full_types))
 
@@ -32,41 +43,47 @@ subsection"Skip"
 text{*In this section we introduce the algebraic laws of programming related to the SKIP
       statement.*}
 
-lemma skip_c_idem [simp]:
+lemma skip_abr_not_ok_left_zero[simp]: 
+  "((\<not>$ok) ;; SKIP\<^sub>A\<^sub>B\<^sub>R) = (\<not>$ok)" 
+  by rel_auto
+
+lemma skip_abr_left_zero[simp]: 
+  "($aburpt ;; SKIP\<^sub>A\<^sub>B\<^sub>R) = $aburpt" 
+  by rel_auto 
+
+lemma skip_abr_bot_left_zero[simp]: 
+  "(\<top>\<^sub>A\<^sub>B\<^sub>R ;; SKIP\<^sub>A\<^sub>B\<^sub>R) = (\<top>\<^sub>A\<^sub>B\<^sub>R)" 
+  by rel_auto
+
+lemma skip_abr_idem [simp]:
   "(SKIP\<^sub>A\<^sub>B\<^sub>R ;; SKIP\<^sub>A\<^sub>B\<^sub>R) = SKIP\<^sub>A\<^sub>B\<^sub>R"
   by rel_auto
 
-lemma skip_c_left_unit[simp]: 
+lemma skip_abr_left_unit[simp]: 
   "(SKIP\<^sub>A\<^sub>B\<^sub>R ;;  Simpl\<^sub>A\<^sub>B\<^sub>R (P)) =  Simpl\<^sub>A\<^sub>B\<^sub>R (P)"
   by rel_auto 
 
-lemma skip_c_right_unit[simp]: 
+lemma skip_abr_right_unit[simp]: 
   "(Simpl\<^sub>A\<^sub>B\<^sub>R (P)  ;;  SKIP\<^sub>A\<^sub>B\<^sub>R) =  Simpl\<^sub>A\<^sub>B\<^sub>R (P)"  
-  by rel_auto (metis option.collapse) 
+  by rel_auto
 
-lemma skip_c_lift_alpha_eq:
+lemma skip_abr_lift_alpha_eq:
   "\<lceil>II\<rceil>\<^sub>A\<^sub>B\<^sub>R = ($\<Sigma>\<^sub>A\<^sub>B\<^sub>R\<acute> =\<^sub>u $\<Sigma>\<^sub>A\<^sub>B\<^sub>R)"
   by rel_auto
 
-lemma skip_c_alpha_eq:
-  "SKIP\<^sub>A\<^sub>B\<^sub>R = Simpl\<^sub>A\<^sub>B\<^sub>R (\<not>$abrupt\<acute> \<and> $abrupt_aux\<acute> =\<^sub>u \<guillemotleft>None\<guillemotright> \<and> ($\<Sigma>\<^sub>A\<^sub>B\<^sub>R\<acute> =\<^sub>u $\<Sigma>\<^sub>A\<^sub>B\<^sub>R))"
-  by (simp add: skip_c_lift_alpha_eq skip_abr_def)
+lemma skip_abr_alpha_eq:
+  "SKIP\<^sub>A\<^sub>B\<^sub>R = Simpl\<^sub>A\<^sub>B\<^sub>R (\<not>$abrupt\<acute> \<and> ($\<Sigma>\<^sub>A\<^sub>B\<^sub>R\<acute> =\<^sub>u $\<Sigma>\<^sub>A\<^sub>B\<^sub>R))"
+  by (simp add: skip_abr_lift_alpha_eq skip_abr_def)
 
-lemma pre_skip_c_post: 
+lemma pre_skip_abr_post: 
   "(Simpl\<^sub>A\<^sub>B\<^sub>R \<lceil>b\<rceil>\<^sub>A\<^sub>B\<^sub>R\<^sub>< \<and> SKIP\<^sub>A\<^sub>B\<^sub>R) = (SKIP\<^sub>A\<^sub>B\<^sub>R \<and> Simpl\<^sub>A\<^sub>B\<^sub>R \<lceil>b\<rceil>\<^sub>A\<^sub>B\<^sub>R\<^sub>>)"
   by rel_auto 
 
-lemma skip_c_var:
-  fixes x :: "(bool,  ('a, 'b) cpa) uvar"
+lemma skip_abr_var:
+  fixes x :: "(bool,  ('b) cpa) uvar"
   shows "(Simpl\<^sub>A\<^sub>B\<^sub>R $x \<and> SKIP\<^sub>A\<^sub>B\<^sub>R) = (SKIP\<^sub>A\<^sub>B\<^sub>R \<and> Simpl\<^sub>A\<^sub>B\<^sub>R $x\<acute>)"
   by rel_auto
 
-lemma assigns_c_id [simp]: "\<langle>id\<rangle>\<^sub>A\<^sub>B\<^sub>R = SKIP\<^sub>A\<^sub>B\<^sub>R"
-  by (rel_auto)
-
-lemma assign_c_alt_def [symbolic_exec_cp]: 
-  "\<langle>\<sigma>\<rangle>\<^sub>A\<^sub>B\<^sub>R = Simpl\<^sub>A\<^sub>B\<^sub>R (\<not>$abrupt\<acute> \<and> $abrupt_aux\<acute> =\<^sub>u \<guillemotleft>None\<guillemotright> \<and> \<lceil>\<lceil>\<sigma>\<rceil>\<^sub>s \<dagger> II\<rceil>\<^sub>A\<^sub>B\<^sub>R)"
-  by rel_auto
 
 subsection {*Assignment Laws*}
 text{*In this section we introduce the algebraic laws of programming related to the assignment
@@ -83,6 +100,13 @@ lemma usubst_c_lift_cancel[usubst,symbolic_exec_cp]:
   shows "\<lceil>($v)\<lbrakk>\<lceil>expr\<rceil>\<^sub></$v\<rbrakk>\<rceil>\<^sub>A\<^sub>B\<^sub>R= \<lceil>expr\<rceil>\<^sub>A\<^sub>B\<^sub>R\<^sub><"
   using 1
   by  rel_auto
+
+lemma assigns_c_id [simp]: "\<langle>id\<rangle>\<^sub>A\<^sub>B\<^sub>R = SKIP\<^sub>A\<^sub>B\<^sub>R"
+  by (rel_auto)
+
+lemma assign_c_alt_def [symbolic_exec_cp]: 
+  "\<langle>\<sigma>\<rangle>\<^sub>A\<^sub>B\<^sub>R = Simpl\<^sub>A\<^sub>B\<^sub>R (\<not>$abrupt\<acute> \<and> \<lceil>\<lceil>\<sigma>\<rceil>\<^sub>s \<dagger> II\<rceil>\<^sub>A\<^sub>B\<^sub>R)"
+  by rel_auto
 
 lemma assigns_c_comp: "(\<langle>f\<rangle>\<^sub>A\<^sub>B\<^sub>R ;; \<langle>g\<rangle>\<^sub>A\<^sub>B\<^sub>R) = \<langle>g \<circ> f\<rangle>\<^sub>A\<^sub>B\<^sub>R"
   by rel_auto 
@@ -117,12 +141,13 @@ proof -
     using assigns_c_comp assigns_c_def utp_urel_laws.assigns_comp
     by metis
 qed
-  
+
 lemma assign_c_cond_c[symbolic_exec_cp]:
   fixes x :: "('a, '\<alpha>) uvar"
   shows "(x \<Midarrow> e ;; (bif b then P else Q eif)) = 
          (bif (b\<lbrakk>e/x\<rbrakk>) then (x \<Midarrow> e ;; P)  else (x \<Midarrow> e ;; Q) eif)"
-  by rel_auto (blast)+
+  apply rel_auto
+oops
 
 lemma assign_c_uop1[symbolic_exec_cp]: 
   assumes 1: "mwb_lens v"
