WP1-Programming-Languages-Semantics/WP11-C-semantics/src/IMP-Lenses/hoare/algebraic_laws_abrupt_aux.thy
@@ -5,6 +5,165 @@ imports "../theories/utp_abrupt_designs"
 
 begin
 
+subsection {*Unrestriction behavior*}
+
+lemma unrest_pre_out\<alpha>_abr [unrest]: "out\<alpha> \<sharp> \<lceil>b\<rceil>\<^sub>A\<^sub>B\<^sub>R\<^sub><"
+  by (transfer, auto simp add: out\<alpha>_def lens_prod_def)
+ 
+lemma unrest_post_in\<alpha>_abr [unrest]: "in\<alpha> \<sharp> \<lceil>b\<rceil>\<^sub>A\<^sub>B\<^sub>R\<^sub>>"
+  by (transfer, auto simp add: in\<alpha>_def lens_prod_def)
+
+lemma unrest_ok_abrupt_lift_rel_uexpr_cpa [unrest]:
+  "$ok \<sharp> \<lceil>P\<rceil>\<^sub>A\<^sub>B\<^sub>R" "$ok\<acute> \<sharp> \<lceil>P\<rceil>\<^sub>A\<^sub>B\<^sub>R"
+  "$abrupt \<sharp> \<lceil>P\<rceil>\<^sub>A\<^sub>B\<^sub>R" "$abrupt\<acute> \<sharp> \<lceil>P\<rceil>\<^sub>A\<^sub>B\<^sub>R"
+  by (pred_auto)+
+
+lemma unrest_ok_abrupt_lift_usubst_cpa [unrest]:
+  "$ok\<acute> \<sharp> \<lceil>\<sigma>\<rceil>\<^sub>s\<^sub>A\<^sub>B\<^sub>R" "$ok \<sharp> \<lceil>\<sigma>\<rceil>\<^sub>s\<^sub>A\<^sub>B\<^sub>R"
+  "$abrupt\<acute> \<sharp> \<lceil>\<sigma>\<rceil>\<^sub>s\<^sub>A\<^sub>B\<^sub>R" "$abrupt \<sharp> \<lceil>\<sigma>\<rceil>\<^sub>s\<^sub>A\<^sub>B\<^sub>R"               
+  by rel_auto+
+
+lemma unrest_ok_abrupt_lift_rel_usubst_cpa [unrest]:
+  "$ok\<acute> \<sharp> \<lceil>\<sigma>\<rceil>\<^sub>S\<^sub>A\<^sub>B\<^sub>R" "$ok \<sharp> \<lceil>\<sigma>\<rceil>\<^sub>S\<^sub>A\<^sub>B\<^sub>R"
+  "$abrupt\<acute> \<sharp> \<lceil>\<sigma>\<rceil>\<^sub>S\<^sub>A\<^sub>B\<^sub>R" "$abrupt \<sharp> \<lceil>\<sigma>\<rceil>\<^sub>S\<^sub>A\<^sub>B\<^sub>R"               
+  by rel_auto+
+
+lemma unrest_pre_in_var_abr [unrest]:
+  "$abrupt \<sharp> \<lceil>p1\<rceil>\<^sub>A\<^sub>B\<^sub>R\<^sub><" " $ok \<sharp> \<lceil>p1\<rceil>\<^sub>A\<^sub>B\<^sub>R\<^sub><"
+  "$abrupt \<sharp> \<lceil>p1\<rceil>\<^sub>A\<^sub>B\<^sub>R\<^sub>>" " $ok \<sharp> \<lceil>p1\<rceil>\<^sub>A\<^sub>B\<^sub>R\<^sub>>"
+  by (transfer, simp)+
+ 
+lemma unrest_in_out_rel_ok_abrupt_res_abr [unrest]:
+  "$ok \<sharp> (P \<restriction>\<^sub>\<alpha> ok)" "$ok\<acute> \<sharp> (P \<restriction>\<^sub>\<alpha> ok)"  
+  "$abrupt \<sharp> (P \<restriction>\<^sub>\<alpha> abrupt)" "$abrupt\<acute> \<sharp> (P \<restriction>\<^sub>\<alpha> abrupt)"
+  by (simp_all add: rel_var_res_def unrest)
+
+subsection {*Substitution behavior*}
+
+lemma seqr_abrupt_true [usubst]: "(P ;; Q) \<^sub>a\<^sub>t = (P \<^sub>a\<^sub>t ;; Q)"
+  by (rel_auto)
+
+lemma seqr_abrupt_false [usubst]: "(P ;; Q) \<^sub>a\<^sub>f = (P \<^sub>a\<^sub>f ;; Q)"
+  by (rel_auto)
+
+lemma bool_seqr_laws_ok [usubst]:
+    "\<And> P Q \<sigma>. \<sigma>($ok \<mapsto>\<^sub>s true) \<dagger> (P ;; Q) = \<sigma> \<dagger> (P\<lbrakk>true/$ok\<rbrakk> ;; Q)"
+    "\<And> P Q \<sigma>. \<sigma>($ok \<mapsto>\<^sub>s false) \<dagger> (P ;; Q) = \<sigma> \<dagger> (P\<lbrakk>false/$ok\<rbrakk> ;; Q)"
+    "\<And> P Q \<sigma>. \<sigma>($ok\<acute> \<mapsto>\<^sub>s true) \<dagger> (P ;; Q) = \<sigma> \<dagger> (P ;; Q\<lbrakk>true/$ok\<acute>\<rbrakk>)"
+    "\<And> P Q \<sigma>. \<sigma>($ok\<acute> \<mapsto>\<^sub>s false) \<dagger> (P ;; Q) = \<sigma> \<dagger> (P ;; Q\<lbrakk>false/$ok\<acute>\<rbrakk>)"
+    by (simp_all add: bool_seqr_laws)
+
+lemma bool_seqr_laws_abrupt [usubst]:
+    "\<And> P Q \<sigma>. \<sigma>($abrupt \<mapsto>\<^sub>s true) \<dagger> (P ;; Q) = \<sigma> \<dagger> (P\<lbrakk>true/$abrupt\<rbrakk> ;; Q)"
+    "\<And> P Q \<sigma>. \<sigma>($abrupt \<mapsto>\<^sub>s false) \<dagger> (P ;; Q) = \<sigma> \<dagger> (P\<lbrakk>false/$abrupt\<rbrakk> ;; Q)"
+    "\<And> P Q \<sigma>. \<sigma>($abrupt\<acute> \<mapsto>\<^sub>s true) \<dagger> (P ;; Q) = \<sigma> \<dagger> (P ;; Q\<lbrakk>true/$abrupt\<acute>\<rbrakk>)"
+    "\<And> P Q \<sigma>. \<sigma>($abrupt\<acute> \<mapsto>\<^sub>s false) \<dagger> (P ;; Q) = \<sigma> \<dagger> (P ;; Q\<lbrakk>false/$abrupt\<acute>\<rbrakk>)"
+    by (simp_all add: bool_seqr_laws)
+
+lemma cpa_ord [usubst]:
+  "$ok \<prec>\<^sub>v $ok\<acute>" "$abrupt \<prec>\<^sub>v $abrupt\<acute>" 
+  "$ok \<prec>\<^sub>v $abrupt\<acute>" "$ok \<prec>\<^sub>v $abrupt" "$ok\<acute> \<prec>\<^sub>v $abrupt\<acute>" "$ok\<acute> \<prec>\<^sub>v $abrupt" 
+  by (simp_all add: var_name_ord_def)
+
+lemma usubst_C3_abr [usubst]: 
+  "\<sigma> \<dagger> C3_abr(P) = (\<sigma> \<dagger> P \<triangleleft> \<sigma> \<dagger> (\<not>$abrupt) \<triangleright> \<sigma> \<dagger> II) "
+  unfolding C3_abr_def usubst_condr .. 
+
+lemma usubst_Simpl_abr [usubst]: 
+  "\<sigma> \<dagger> Simpl\<^sub>A\<^sub>B\<^sub>R (P) = (\<sigma> \<dagger> (\<lceil>true\<rceil>\<^sub>A\<^sub>B\<^sub>R \<turnstile> P) \<triangleleft> \<sigma> \<dagger> (\<not>$abrupt) \<triangleright> \<sigma> \<dagger> II)"
+  unfolding C3_abr_def usubst_condr ..
+
+lemma usubst_lift_pre_uexpr_cpa[simp]:
+  "\<lceil>\<sigma>\<rceil>\<^sub>s\<^sub>A\<^sub>B\<^sub>R \<dagger> \<lceil>b\<rceil>\<^sub>A\<^sub>B\<^sub>R\<^sub>< = \<lceil>\<sigma> \<dagger> b\<rceil>\<^sub>A\<^sub>B\<^sub>R\<^sub><" 
+  by rel_auto
+
+lemma rel_usubst_lift_pre_uexpr_cpa[simp]:
+  "\<lceil>\<sigma>\<rceil>\<^sub>S\<^sub>A\<^sub>B\<^sub>R \<dagger> \<lceil>b\<rceil>\<^sub>A\<^sub>B\<^sub>R\<^sub>< = \<lceil>\<sigma> \<dagger> \<lceil>b\<rceil>\<^sub><\<rceil>\<^sub>A\<^sub>B\<^sub>R" 
+  by rel_auto
+
+lemma rel_usubst_lift_post_uexpr_cpa[simp]:
+  "\<lceil>\<sigma>\<rceil>\<^sub>S\<^sub>A\<^sub>B\<^sub>R \<dagger> \<lceil>b\<rceil>\<^sub>A\<^sub>B\<^sub>R\<^sub>> = \<lceil>\<sigma> \<dagger> \<lceil>b\<rceil>\<^sub>>\<rceil>\<^sub>A\<^sub>B\<^sub>R" 
+  by rel_auto
+
+lemma usubst_cond_abr[usubst]:
+  "\<lceil>\<sigma>\<rceil>\<^sub>s\<^sub>A\<^sub>B\<^sub>R \<dagger> (bif b then P else Q eif) = 
+   ((\<lceil>\<sigma>\<rceil>\<^sub>s\<^sub>A\<^sub>B\<^sub>R \<dagger> \<lceil>true\<rceil>\<^sub>A\<^sub>B\<^sub>R \<turnstile> (\<lceil>\<sigma>\<rceil>\<^sub>s\<^sub>A\<^sub>B\<^sub>R \<dagger> P \<triangleleft> \<lceil>\<sigma> \<dagger> b\<rceil>\<^sub>A\<^sub>B\<^sub>R\<^sub>< \<triangleright> \<lceil>\<sigma>\<rceil>\<^sub>s\<^sub>A\<^sub>B\<^sub>R \<dagger> Q)) \<triangleleft> \<lceil>\<sigma>\<rceil>\<^sub>s\<^sub>A\<^sub>B\<^sub>R \<dagger> (\<not> $abrupt) \<triangleright> \<lceil>\<sigma>\<rceil>\<^sub>s\<^sub>A\<^sub>B\<^sub>R \<dagger> II)"
+   unfolding C3_abr_def
+  by (simp add: usubst unrest)
+
+lemma usubst_cpa_des_cond_abr [usubst]:
+  "\<lbrakk>$ok \<sharp> \<sigma>; $ok\<acute> \<sharp> \<sigma> \<rbrakk> \<Longrightarrow> 
+    \<sigma> \<dagger> (\<lceil>true\<rceil>\<^sub>A\<^sub>B\<^sub>R \<turnstile> bif b then P else Q eif) = 
+    (\<sigma> \<dagger> \<lceil>true\<rceil>\<^sub>A\<^sub>B\<^sub>R \<turnstile>  ((\<sigma> \<dagger> \<lceil>true\<rceil>\<^sub>A\<^sub>B\<^sub>R \<turnstile> (\<sigma> \<dagger> P \<triangleleft> \<sigma> \<dagger> \<lceil>b\<rceil>\<^sub>A\<^sub>B\<^sub>R\<^sub>< \<triangleright> \<sigma> \<dagger> Q)) \<triangleleft> \<sigma> \<dagger> (\<not> $abrupt) \<triangleright> \<sigma> \<dagger> II))"
+  by (simp add: usubst)
+
+lemma usubst_rel_des_cond_abr [usubst]:
+  "\<lceil>\<sigma>\<rceil>\<^sub>S\<^sub>A\<^sub>B\<^sub>R \<dagger> (\<lceil>true\<rceil>\<^sub>A\<^sub>B\<^sub>R \<turnstile> bif b then P else Q eif) = 
+   (\<lceil>\<sigma>\<rceil>\<^sub>S\<^sub>A\<^sub>B\<^sub>R \<dagger> \<lceil>true\<rceil>\<^sub>A\<^sub>B\<^sub>R \<turnstile>  ((\<lceil>\<sigma>\<rceil>\<^sub>S\<^sub>A\<^sub>B\<^sub>R \<dagger> \<lceil>true\<rceil>\<^sub>A\<^sub>B\<^sub>R \<turnstile> (\<lceil>\<sigma>\<rceil>\<^sub>S\<^sub>A\<^sub>B\<^sub>R \<dagger> P \<triangleleft> \<lceil>\<sigma> \<dagger> \<lceil>b\<rceil>\<^sub><\<rceil>\<^sub>A\<^sub>B\<^sub>R \<triangleright> \<lceil>\<sigma>\<rceil>\<^sub>S\<^sub>A\<^sub>B\<^sub>R \<dagger> Q)) \<triangleleft> \<lceil>\<sigma>\<rceil>\<^sub>S\<^sub>A\<^sub>B\<^sub>R \<dagger> (\<not> $abrupt) \<triangleright> \<lceil>\<sigma>\<rceil>\<^sub>S\<^sub>A\<^sub>B\<^sub>R \<dagger> II))"
+  by (simp add: usubst unrest)
+
+lemma usubst_des_cond_abr [usubst]:   
+  "\<lceil>\<sigma>\<rceil>\<^sub>s\<^sub>A\<^sub>B\<^sub>R \<dagger> (\<lceil>true\<rceil>\<^sub>A\<^sub>B\<^sub>R \<turnstile> bif b then P else Q eif) = 
+   (\<lceil>\<sigma>\<rceil>\<^sub>s\<^sub>A\<^sub>B\<^sub>R \<dagger> \<lceil>true\<rceil>\<^sub>A\<^sub>B\<^sub>R \<turnstile>  ((\<lceil>\<sigma>\<rceil>\<^sub>s\<^sub>A\<^sub>B\<^sub>R \<dagger> \<lceil>true\<rceil>\<^sub>A\<^sub>B\<^sub>R \<turnstile> (\<lceil>\<sigma>\<rceil>\<^sub>s\<^sub>A\<^sub>B\<^sub>R \<dagger> P \<triangleleft> \<lceil>\<sigma>\<rceil>\<^sub>s\<^sub>A\<^sub>B\<^sub>R \<dagger> \<lceil>b\<rceil>\<^sub>A\<^sub>B\<^sub>R\<^sub>< \<triangleright> \<lceil>\<sigma>\<rceil>\<^sub>s\<^sub>A\<^sub>B\<^sub>R \<dagger> Q)) \<triangleleft> \<lceil>\<sigma>\<rceil>\<^sub>s\<^sub>A\<^sub>B\<^sub>R \<dagger> (\<not> $abrupt) \<triangleright> \<lceil>\<sigma>\<rceil>\<^sub>s\<^sub>A\<^sub>B\<^sub>R \<dagger> II))"
+  by (simp add: usubst unrest)
+
+subsection {*Assign abrupt behavior*}
+
+lemma assigns_usubst_cpa [usubst] :
+  "\<lceil>\<sigma>\<rceil>\<^sub>s\<^sub>A\<^sub>B\<^sub>R \<dagger> \<lceil>\<langle>\<rho>\<rangle>\<^sub>a\<rceil>\<^sub>A\<^sub>B\<^sub>R = \<lceil>\<langle>\<rho> \<circ> \<sigma>\<rangle>\<^sub>a\<rceil>\<^sub>A\<^sub>B\<^sub>R" 
+  by rel_auto
+
+lemma assigns_cpa_comp:
+   "\<lbrakk>$ok \<sharp> P; $ok\<acute> \<sharp> P; $abrupt \<sharp> P; $abrupt\<acute> \<sharp> P\<rbrakk>\<Longrightarrow> 
+   (\<lceil>\<langle>\<sigma>\<rangle>\<^sub>a\<rceil>\<^sub>A\<^sub>B\<^sub>R ;; P) = (\<lceil>\<sigma>\<rceil>\<^sub>s\<^sub>A\<^sub>B\<^sub>R \<dagger> P)"
+   apply pred_auto apply transfer 
+   apply (metis cp_abr.surjective des_vars.surjective des_vars_ext_def fst_conv in\<alpha>_def lens.select_convs(1) lens.select_convs(2) old.prod.case snd_conv)
+   apply transfer
+   apply (smt cp_abr.simps(2) cp_abr_ext_def des_vars.select_convs(2) des_vars_ext_def fst_conv in\<alpha>_def lens.select_convs(1) lens.select_convs(2) mem_Collect_eq old.prod.case relcomp.simps snd_conv) 
+done
+ 
+lemma assigns_cpa_rel_lift_comp: 
+  "(\<lceil>\<langle>\<sigma>\<rangle>\<^sub>a\<rceil>\<^sub>A\<^sub>B\<^sub>R ;; \<lceil>P\<rceil>\<^sub>A\<^sub>B\<^sub>R) = (\<lceil>\<sigma>\<rceil>\<^sub>s\<^sub>A\<^sub>B\<^sub>R \<dagger> \<lceil>P\<rceil>\<^sub>A\<^sub>B\<^sub>R)"
+  by rel_auto 
+
+thm assigns_subst
+
+lemma "\<lceil>\<sigma>\<rceil>\<^sub>S\<^sub>A\<^sub>B\<^sub>R \<dagger> \<langle>\<rho>\<rangle>\<^sub>A\<^sub>B\<^sub>R = \<langle>\<rho> \<circ> \<lfloor>\<sigma>\<rfloor>\<^sub>s\<rangle>\<^sub>A\<^sub>B\<^sub>R" 
+  apply transfer apply rel_auto oops
+term "\<lceil>\<langle>\<rho> \<circ> \<sigma>\<rangle>\<^sub>a\<rceil>\<^sub>A\<^sub>B\<^sub>R"
+
+
+lemma assigns_abr_subst [usubst]:
+  " \<lceil>\<sigma>\<rceil>\<^sub>s\<^sub>A\<^sub>B\<^sub>R \<dagger> \<langle>\<rho>\<rangle>\<^sub>A\<^sub>B\<^sub>R = \<langle>\<rho> \<circ> \<sigma>\<rangle>\<^sub>A\<^sub>B\<^sub>R"
+  apply transfer  apply (rel_auto) oops
+
+lemma assigns_abr_comp: "(\<langle>f\<rangle>\<^sub>A\<^sub>B\<^sub>R ;; \<langle>g\<rangle>\<^sub>A\<^sub>B\<^sub>R) = \<langle>g \<circ> f\<rangle>\<^sub>A\<^sub>B\<^sub>R"
+  by rel_auto 
+thm design_composition
+
+lemma assign_d_left_comp:
+assumes
+    "$ok\<acute> \<sharp> (P \<turnstile> Q)" "$ok \<sharp> (P \<turnstile> Q)" 
+  shows
+  "(\<langle>f\<rangle>\<^sub>A\<^sub>B\<^sub>R ;; (P \<turnstile> Q)) = (\<lceil>\<lceil>f\<rceil>\<^sub>s\<rceil>\<^sub>A\<^sub>B \<dagger> P \<turnstile> \<lceil>\<lceil>f\<rceil>\<^sub>s\<rceil>\<^sub>A\<^sub>B \<dagger> Q)"
+  apply (simp add: assigns_c_def    C3_abr_def)
+
+lemma assign_d_right_comp:
+  "((P \<turnstile>\<^sub>r Q) ;; \<langle>f\<rangle>\<^sub>D) = ((\<not> ((\<not> P) ;; true)) \<turnstile>\<^sub>r (Q ;; \<langle>f\<rangle>\<^sub>a))"
+  by (simp add: assigns_d_def rdesign_composition)
+
+lemma assigns_d_comp:
+  "(\<langle>f\<rangle>\<^sub>D ;; \<langle>g\<rangle>\<^sub>D) = \<langle>g \<circ> f\<rangle>\<^sub>D"
+  by (simp add: assigns_d_def rdesign_composition assigns_comp)
+
+subsection {*Seq behavior*}
+
+lemma lift_des_skip_dr_unit_abr [simp]:
+  "(\<lceil>P\<rceil>\<^sub>A\<^sub>B\<^sub>R ;; \<lceil>II\<rceil>\<^sub>A\<^sub>B\<^sub>R) = \<lceil>P\<rceil>\<^sub>A\<^sub>B\<^sub>R"
+  "(\<lceil>II\<rceil>\<^sub>A\<^sub>B\<^sub>R ;; \<lceil>P\<rceil>\<^sub>A\<^sub>B\<^sub>R) = \<lceil>P\<rceil>\<^sub>A\<^sub>B\<^sub>R"
+  by (rel_auto)+
+
+
 subsection {*Abrupt semantics behavior*}
 
 lemma Simpl_abr_idem[simp]: "Simpl\<^sub>A\<^sub>B\<^sub>R(Simpl\<^sub>A\<^sub>B\<^sub>R(P)) = Simpl\<^sub>A\<^sub>B\<^sub>R(P)"
@@ -36,18 +195,18 @@ lemma Simpl_abr_throw_abr[simp]: "Simpl\<^sub>A\<^sub>B\<^sub>R(THROW\<^sub>A\<^
 lemma Simpl_abr_assign_abr[simp]: "Simpl\<^sub>A\<^sub>B\<^sub>R(\<langle>\<sigma>\<rangle>\<^sub>A\<^sub>B\<^sub>R) = (\<langle>\<sigma>\<rangle>\<^sub>A\<^sub>B\<^sub>R)"
   by (rel_auto)
 
-lemma Simpl_abr_form: "Simpl\<^sub>A\<^sub>B\<^sub>R(P) = ((\<not> (\<not>$abrupt \<and> ($abrupt_aux =\<^sub>u \<guillemotleft>None\<guillemotright>)) \<and> II) \<or> 
-                              (\<not>$abrupt \<and> $abrupt_aux =\<^sub>u \<guillemotleft>None\<guillemotright> \<and> (\<lceil>true\<rceil>\<^sub>A\<^sub>B\<^sub>R \<turnstile> (P))))"
+lemma Simpl_abr_form: "
+  Simpl\<^sub>A\<^sub>B\<^sub>R(P) = ((\<not> (\<not>$abrupt) \<and> II) \<or> ((\<not>$abrupt) \<and> (\<lceil>true\<rceil>\<^sub>A\<^sub>B\<^sub>R \<turnstile> (P))))"
   by (rel_auto) 
 
 lemma abrupt_Simpl_abr:
-  "(\<not> (\<not>$abrupt \<and> ($abrupt_aux =\<^sub>u \<guillemotleft>None\<guillemotright>)) \<and> Simpl\<^sub>A\<^sub>B\<^sub>R(P)) = 
-   (II \<and> \<not> (\<not>$abrupt\<acute> \<and> ($abrupt_aux\<acute> =\<^sub>u \<guillemotleft>None\<guillemotright>)))"
+  "(\<not> (\<not>$abrupt ) \<and> Simpl\<^sub>A\<^sub>B\<^sub>R(P)) = 
+   (II \<and> \<not> (\<not>$abrupt\<acute>))"
   by (rel_auto)
 
 lemma nabrupt_Simpl_abr:
-  "(\<not>$abrupt \<and> $abrupt_aux =\<^sub>u \<guillemotleft>None\<guillemotright> \<and> Simpl\<^sub>A\<^sub>B\<^sub>R(P)) = 
-   (\<not>$abrupt \<and> $abrupt_aux =\<^sub>u \<guillemotleft>None\<guillemotright> \<and> (\<lceil>true\<rceil>\<^sub>A\<^sub>B\<^sub>R \<turnstile> (P)))"
+  "(\<not>$abrupt \<and> \<not>$fault \<and> Simpl\<^sub>A\<^sub>B\<^sub>R(P)) = 
+   (\<not>$abrupt \<and>\<not>$fault \<and> (\<lceil>true\<rceil>\<^sub>A\<^sub>B\<^sub>R \<turnstile> (P)))"
   by (rel_auto)
 
 lemma Simpl_abr_semir_form:
@@ -60,7 +219,7 @@ lemma Simpl_abr_semir_closure:
   using assms
   by (metis  Healthy_def Simpl_abr_semir_form Simpl_abr_idem)
 
-definition design_abr_sup :: "('a,'\<alpha>,'\<beta>) rel_cpa set \<Rightarrow> ('a,'\<alpha>,'\<beta>) rel_cpa" ("\<Sqinter>\<^sub>A\<^sub>B\<^sub>R_" [900] 900) where
+definition design_abr_sup :: "('\<alpha>,'\<beta>) rel_cpa set \<Rightarrow> ('\<alpha>,'\<beta>) rel_cpa" ("\<Sqinter>\<^sub>A\<^sub>B\<^sub>R_" [900] 900) where
 "\<Sqinter>\<^sub>A\<^sub>B\<^sub>R A = (if (A = {}) then \<top>\<^sub>A\<^sub>B\<^sub>R else \<Sqinter> A)"
 
 lemma Simpl_abr_Continuous: "Continuous Simpl\<^sub>A\<^sub>B\<^sub>R"
